StringRewriting/Basic.lean
@@ -4,6 +4,6 @@ variable {Symbol : Type} [Inhabited Symbol] [Fintype Symbol]
 
 open Turing SingleTapeTM
 
-variable {M : SingleTapeTM Symbol}
-variable {N : SingleTapeTM Symbol}
+variable {m : SingleTapeTM Symbol}
+variable {n : SingleTapeTM Symbol}
 
